Tidy up

examples/steel/ProductPCM.fst
@@ -79,40 +79,15 @@ let tuple_comp p q (xa, xb) (ya, yb) = composable p xa ya /\ composable q xb yb
 val tuple_op : p: pcm 'a -> q: pcm 'b -> x:('a & 'b) -> y:('a & 'b){tuple_comp p q x y} -> 'a & 'b
 let tuple_op p q (xa, xb) (ya, yb) = (op p xa ya, op q xb yb)
 
-// val full : pcm' 'a -> 'a -> prop
-// let full #a p x = forall (frame:a{p.composable frame x}). p.op frame x == x
-
-(* This product construction needs some additional assumptions in order to work: *)
-noeq type refined_pcm a = {
-  u: pcm a;
-  (* The unit is the unique "least element" of the preorder defined by
-     [compatible]. (i.e., nothing can be "inside of" or "have less
-     information than" the unit of the PCM) *)
-  compat_unit_unique : x:a ->
-    Lemma (compatible u x u.p.one ==> x == u.p.one);
-// (* refine says that an element is either unit or a full value *)
-// refine_unit_or_full : x:a ->
-//   Lemma (u.refine x == (x == u.p.one \/ full u.p x));
+val tuple_pcm : pcm 'a -> pcm 'b -> pcm ('a & 'b)
+let tuple_pcm #a #b p q = {
+  p = {composable = tuple_comp p q; op = tuple_op p q; one = (p.p.one, q.p.one)};
+  comm = (fun (xa, xb) (ya, yb) -> p.comm xa ya; q.comm xb yb);
+  assoc = (fun (xa, xb) (ya, yb) (za, zb) -> p.assoc xa ya za; q.assoc xb yb zb);
+  assoc_r = (fun (xa, xb) (ya, yb) (za, zb) -> p.assoc_r xa ya za; q.assoc_r xb yb zb);
+  is_unit = (fun (xa, xb) -> p.is_unit xa; q.is_unit xb);
+  refine = (fun (xa, xb) -> p.refine xa /\ q.refine xb)
 }
-  
-val tuple_pcm : refined_pcm 'a -> refined_pcm 'b -> refined_pcm ('a & 'b)
-let tuple_pcm #a #b p q =
-  let p' = FStar.PCM.({
-    composable = tuple_comp p.u q.u;
-    op = tuple_op p.u q.u;
-    one = (p.u.p.one, q.u.p.one)
-  }) in
-  let u = FStar.PCM.({
-    p = p';
-    comm = (fun (xa, xb) (ya, yb) -> p.u.comm xa ya; q.u.comm xb yb);
-    assoc = (fun (xa, xb) (ya, yb) (za, zb) -> p.u.assoc xa ya za; q.u.assoc xb yb zb);
-    assoc_r = (fun (xa, xb) (ya, yb) (za, zb) -> p.u.assoc_r xa ya za; q.u.assoc_r xb yb zb);
-    is_unit = (fun (xa, xb) -> p.u.is_unit xa; q.u.is_unit xb);
-    refine = (fun (xa, xb) -> (xa, xb) == p'.one \/ (p.u.refine xa /\ q.u.refine xb))
-  }) in {
-    u = u;
-    compat_unit_unique = (fun (xa, xb) -> p.compat_unit_unique xa; q.compat_unit_unique xb)
-  }
 
 open Steel.Memory
 open Steel.Effect.Atomic
@@ -125,123 +100,35 @@ module T = FStar.Tactics
 /// tuple PCM from frame-preserving updates on its components:
 
 val compatible_tuple_l :
-  p: refined_pcm 'a -> q: refined_pcm 'b ->
+  p: pcm 'a -> q: pcm 'b ->
   x: 'a -> v: 'a -> y: 'b -> w: 'b ->
   Lemma 
-    (requires compatible p.u x v /\ compatible q.u y w)
-    (ensures compatible (tuple_pcm p q).u (x, y) (v, w))
+    (requires compatible p x v /\ compatible q y w)
+    (ensures compatible (tuple_pcm p q) (x, y) (v, w))
 let compatible_tuple_l p q x v y w =
-  let pqu = (tuple_pcm p q).u in
+  let pq = tuple_pcm p q in
   let aux frame_x frame_y :
     Lemma 
-      (requires composable pqu (x, y) (frame_x, frame_y) /\
-                op pqu (frame_x, frame_y) (x, y) == (v, w))
-      (ensures compatible pqu (x, y) (v, w))
-      [SMTPat (composable p.u x frame_x); SMTPat (composable q.u y frame_y)] =
-    ()
+      (requires composable pq (x, y) (frame_x, frame_y) /\
+                op pq (frame_x, frame_y) (x, y) == (v, w))
+      (ensures compatible pq (x, y) (v, w))
+      [SMTPat (composable p x frame_x); SMTPat (composable q y frame_y)] = ()
   in ()
 
 val upd_fst :
-  p: refined_pcm 'a -> q: refined_pcm 'b ->
-  x: 'a {~ (x == p.u.p.one)} -> y: 'b -> x': 'a ->
-  frame_preserving_upd p.u x x' ->
-  frame_preserving_upd (tuple_pcm p q).u (x, y) (x', y)
+  p: pcm 'a -> q: pcm 'b ->
+  x: 'a -> y: 'b -> x': 'a ->
+  frame_preserving_upd p x x' ->
+  frame_preserving_upd (tuple_pcm p q) (x, y) (x', y)
 let upd_fst #a #b p q x y x' f (va, vb) =
-  p.compat_unit_unique x;
   let wa = f va in
-  let pqu = (tuple_pcm p q).u in
+  let pq = tuple_pcm p q in
   compatible_tuple_l p q x' wa y vb;
-  let lemma (frame: (a & b) {composable pqu (x, y) frame}):
-    Lemma (composable pqu (x', y) frame /\
-           (op pqu (x, y) frame == (va, vb) ==> op pqu (x', y) frame == (wa, vb)))
-    [SMTPat (composable pqu (x, y) frame)] = ()
+  let lemma (frame: (a & b) {composable pq (x, y) frame}):
+    Lemma (composable pq (x', y) frame /\
+           (op pq (x, y) frame == (va, vb) ==> op pq (x', y) frame == (wa, vb)))
+    [SMTPat (composable pq (x, y) frame)] = ()
   in (wa, vb)
-
-(*
-val upd_fst_0 :
-  p: refined_pcm 'a -> q: refined_pcm 'b ->
-  r: ref ('a & 'b) (tuple_pcm p q).u ->
-  x: Ghost.erased 'a {~ (Ghost.reveal x == p.u.p.one)} -> y: Ghost.erased 'b -> x': 'a ->
-  frame_preserving_upd p.u x x' ->
-  frame_preserving_upd (tuple_pcm p q).u (Ghost.reveal x, Ghost.reveal y) (x', Ghost.reveal y)
-let upd_fst_0 p q r x y x' upd_x (vx, vy) =
-  assume (compatible (tuple_pcm p q).u (x', Ghost.reveal y) (upd_x vx, vy));
-  // Since x != 1 and compatible x vx, vx != 1 by compat_unit_unique.
-  assert (compatible p.u (Ghost.reveal x) vx);
-  p.compat_unit_unique (Ghost.reveal x);
-  assert (~ (vx == p.u.p.one));
-  // Thus, if refine (vx, vy), vx and vy must be full values.
-  assert ((tuple_pcm p q).u.refine (vx, vy) ==> full (tuple_pcm p q).u.p (vx, vy));
-  full_tup p q vx vy;
-  // A frame-preserving update sends full values to full values, so (upd_x vx, vy) is full too.
-  assume ((tuple_pcm p q).u.refine (vx, vy) ==> full q.u.p vy); (* TODO why doesn't this work? *)
-  assume ((tuple_pcm p q).u.refine (vx, vy) ==> full p.u.p vx); (* TODO why doesn't this work? *)
-  assume (full p.u.p (upd_x vx)); (* can't be unit because upd_x is frame_preserving and vx != unit *)
-  full_tup p q (upd_x vx) vy;
-  assert ((tuple_pcm p q).u.refine (vx, vy) ==> full (tuple_pcm p q).u.p (upd_x vx, vy));
-  assert ((tuple_pcm p q).u.refine (vx, vy) ==> (tuple_pcm p q).u.refine (upd_x vx, vy));
-  assume ((tuple_pcm p q).u.refine (vx, vy) ==> frame_preserving (tuple_pcm p q).u (vx, vy) (upd_x vx, vy));
-  (upd_x vx, vy)
-*)
-
-(*
-val full_tup :
-  p: refined_pcm 'a -> q: refined_pcm 'b -> x: 'a -> y: 'b ->
-  full (tuple_pcm p q).u.p (x, y) == full p.u.p x /\ full q.u.p y
-let full_tup p q x y =
-  (* (forall (x', y') composable with (x, y). (x <> x', y <> y') = (x, y))
-     <=> (forall x' comp w/ x and y' comp w/ y. x <> x' = x /\ y <> y' = y)
-     <=> (forall x' comp w/ x. x <> x' = x) /\ (forall y' comp w/. y <> y' = y) *)
-  admit() (* TODO how to prove this? *)
-  *)
-
-(*
-val frame_preserving_full_value :
-  p: refined_pcm 'a -> x: 'a -> y: 'a ->
-  f:frame_preserving_upd_0 p.u x y ->
-  Lemma (requires full p.u.p x) (ensures full p.u.p (f v))
-let frame_preserving_full_value #a p x y f =
-  compatible_refl p.u x;
-  p.refine_unit_or_full x;
-  assert (p.u.refine x);
-  let z = f x in
-  assert (p.u.refine z);
-  assert (frame_preserving p.u x z);
-  assume (forall (frame:a{composable p.u frame z}). op p.u frame z == z);
-  admit()
-  *)
-
-(*
-val upd_fst_0 :
-  p: refined_pcm 'a -> q: refined_pcm 'b ->
-  r: ref ('a & 'b) (tuple_pcm p q).u ->
-  x: Ghost.erased 'a {~ (Ghost.reveal x == p.u.p.one)} -> y: Ghost.erased 'b -> x': 'a ->
-  frame_preserving_upd_0 p.u x x' ->
-  frame_preserving_upd_0 (tuple_pcm p q).u (Ghost.reveal x, Ghost.reveal y) (x', Ghost.reveal y)
-let upd_fst_0 p q r x y x' upd_x (vx, vy) =
-  assume (compatible (tuple_pcm p q).u (x', Ghost.reveal y) (upd_x vx, vy));
-  // Since x != 1 and compatible x vx, vx != 1 by compat_unit_unique.
-  assert (compatible p.u (Ghost.reveal x) vx);
-  p.compat_unit_unique (Ghost.reveal x);
-  assert (~ (vx == p.u.p.one));
-  // Thus, if refine (vx, vy), vx and vy must be full values.
-  assert ((tuple_pcm p q).u.refine (vx, vy) ==> full (tuple_pcm p q).u.p (vx, vy));
-  full_tup p q vx vy;
-  // A frame-preserving update sends full values to full values, so (upd_x vx, vy) is full too.
-  assume ((tuple_pcm p q).u.refine (vx, vy) ==> full q.u.p vy); (* TODO why doesn't this work? *)
-  assume ((tuple_pcm p q).u.refine (vx, vy) ==> full p.u.p vx); (* TODO why doesn't this work? *)
-  assume (full p.u.p (upd_x vx)); (* can't be unit because upd_x is frame_preserving and vx != unit *)
-  full_tup p q (upd_x vx) vy;
-  assert ((tuple_pcm p q).u.refine (vx, vy) ==> full (tuple_pcm p q).u.p (upd_x vx, vy));
-  assert ((tuple_pcm p q).u.refine (vx, vy) ==> (tuple_pcm p q).u.refine (upd_x vx, vy));
-  assume ((tuple_pcm p q).u.refine (vx, vy) ==> frame_preserving (tuple_pcm p q).u (vx, vy) (upd_x vx, vy));
-  (upd_x vx, vy)
-  *)
-  
-  (*
-  change_slprop (pts_to r (Ghost.reveal x, Ghost.reveal y)) (pts_to r (Ghost.reveal (Ghost.hide (Ghost.reveal x, Ghost.reveal y)))) (fun _ -> ());
-  upd_gen r (Ghost.hide (Ghost.reveal x, Ghost.reveal y)) (Ghost.hide (Ghost.reveal x', Ghost.reveal y)) upd;
-  change_slprop (pts_to r (Ghost.reveal (Ghost.hide (Ghost.reveal x', Ghost.reveal y)))) (pts_to r (Ghost.reveal x', Ghost.reveal y)) (fun _ -> ())*)
 
 /// If no custom PCM is needed, p and q can be instantiated with an all-or-none PCM:
 
@@ -252,117 +139,106 @@ val opt_op : x:option 'a -> y:option 'a {opt_comp x y} -> option 'a
 let opt_op x y = match x, y with None, z | z, None -> z
 
 val opt_pcm : pcm (option 'a)
-let opt_pcm #a = FStar.PCM.({
-  p = {
-    composable=opt_comp;
-    op=opt_op;
-    one=None
-  };
+let opt_pcm #a = {
+  p = {composable = opt_comp; op = opt_op; one = None};
   comm = (fun _ _ -> ());
   assoc = (fun _ _ _ -> ());
   assoc_r = (fun _ _ _ -> ());
   is_unit = (fun _ -> ());
   refine = (fun _ -> True);
-})
+}
 
 /// We can generalize to 'a-ary products (z:'a -> f z), given a PCM for each z:
 
 open FStar.FunctionalExtensionality
 
 val prod_comp :
-  f:('a -> Type) -> (z:'a -> pcm (f z)) ->
+  #f:('a -> Type) -> (z:'a -> pcm (f z)) ->
   restricted_t 'a f -> restricted_t 'a f -> prop
-let prod_comp f p x y = forall z. composable (p z) (x z) (y z)
+let prod_comp p x y = forall z. composable (p z) (x z) (y z)
 
 val prod_op :
-  f:('a -> Type) -> p:(z:'a -> pcm (f z)) -> 
-  x:restricted_t 'a f -> y: restricted_t 'a f {prod_comp f p x y} -> 
+  #f:('a -> Type) -> p:(z:'a -> pcm (f z)) -> 
+  x:restricted_t 'a f -> y: restricted_t 'a f {prod_comp p x y} -> 
   restricted_t 'a f
-let prod_op #a f p x y = on_domain a (fun z -> op (p z) (x z) (y z))
+let prod_op #a p x y = on_domain a (fun z -> op (p z) (x z) (y z))
 
-val prod_one : f:('a -> Type) -> (z:'a -> pcm (f z)) -> restricted_t 'a f
-let prod_one f p = on_domain _ (fun z -> (p z).p.one)
+val prod_one : #f:('a -> Type) -> (z:'a -> pcm (f z)) -> restricted_t 'a f
+let prod_one #a p = on_domain a (fun z -> (p z).p.one)
 
-let ext (a: Type) (b: (a -> Type)) (f g: restricted_t a b)
-  : Lemma (ensures (feq #a #b f g <==> f == g))
-= extensionality a b f g
-
-val prod_pcm' : f:('a -> Type) -> (z:'a -> pcm (f z)) -> pcm' (restricted_t 'a f)
-let prod_pcm' #a f p = FStar.PCM.({
-  composable = prod_comp f p;
-  op = prod_op f p;
-  one = prod_one f p;
-})
+val ext :
+  #b: ('a -> Type) -> f: restricted_t 'a b -> g: restricted_t 'a b -> 
+  (x: 'a -> Lemma (f x == g x)) ->
+  Lemma (ensures (f == g))
+let ext #a #b f g fg =
+  extensionality a b f g;
+  forall_intro fg
 
 val prod_comm :
-  f:('a -> Type) -> p:(z:'a -> pcm (f z)) ->
+  #f:('a -> Type) -> p:(z:'a -> pcm (f z)) ->
   x:restricted_t 'a f ->
-  y:restricted_t 'a f {prod_comp f p x y} ->
-  Lemma (prod_op f p x y == prod_op f p y x)
-let prod_comm #a f p x y =
-  let comm (z:a): Lemma ((p z).p.op (x z) (y z) == (p z).p.op (y z) (x z)) =
-    (p z).comm (x z) (y z)
-  in forall_intro comm;
-  ext a f (prod_op f p x y) (prod_op f p y x)
+  y:restricted_t 'a f {prod_comp p x y} ->
+  Lemma (prod_op p x y == prod_op p y x)
+let prod_comm p x y =
+  ext (prod_op p x y) (prod_op p y x) (fun z -> (p z).comm (x z) (y z))
 
 val prod_assoc :
-  f:('a -> Type) -> p:(w:'a -> pcm (f w)) ->
-  x:restricted_t 'a f ->
-  y:restricted_t 'a f ->
-  z:restricted_t 'a f {prod_comp f p y z /\ prod_comp f p x (prod_op f p y z)} ->
-  Lemma (prod_comp f p x y /\
-         prod_comp f p (prod_op f p x y) z /\
-         prod_op f p x (prod_op f p y z) == prod_op f p (prod_op f p x y) z)
-let prod_assoc #a f p x y z =
-  let assoc (w:a): 
+  #f:('a -> Type) -> p:(w:'a -> pcm (f w)) ->
+  x:restricted_t 'a f -> y:restricted_t 'a f ->
+  z:restricted_t 'a f {prod_comp p y z /\ prod_comp p x (prod_op p y z)} ->
+  Lemma (prod_comp p x y /\
+         prod_comp p (prod_op p x y) z /\
+         prod_op p x (prod_op p y z) == prod_op p (prod_op p x y) z)
+let prod_assoc p x y z =
+  let aux w :
     Lemma (composable (p w) (x w) (y w) /\
-           composable (p w) (op (p w) (x w) (y w)) (z w) /\
-           op (p w) (x w) (op (p w) (y w) (z w)) == op (p w) (op (p w) (x w) (y w)) (z w)) 
-  = (p w).assoc (x w) (y w) (z w) in
-  forall_intro assoc;
-  ext a f (prod_op f p x (prod_op f p y z)) (prod_op f p (prod_op f p x y) z)
+           composable (p w) (op (p w) (x w) (y w)) (z w)) 
+    [SMTPat (p w)] = (p w).assoc (x w) (y w) (z w)
+  in
+  ext (prod_op p x (prod_op p y z)) (prod_op p (prod_op p x y) z)
+    (fun w -> (p w).assoc (x w) (y w) (z w))
 
 val prod_assoc_r :
-  f:('a -> Type) -> p:(w:'a -> pcm (f w)) ->
-  x:restricted_t 'a f ->
-  y:restricted_t 'a f ->
-  z:restricted_t 'a f {prod_comp f p x y /\ prod_comp f p (prod_op f p x y) z} ->
-  Lemma (prod_comp f p y z /\
-         prod_comp f p x (prod_op f p y z) /\
-         prod_op f p x (prod_op f p y z) == prod_op f p (prod_op f p x y) z)
-let prod_assoc_r #a f p x y z =
-  let assoc_r (w:a): 
+  #f:('a -> Type) -> p:(w:'a -> pcm (f w)) ->
+  x:restricted_t 'a f -> y:restricted_t 'a f ->
+  z:restricted_t 'a f {prod_comp p x y /\ prod_comp p (prod_op p x y) z} ->
+  Lemma (prod_comp p y z /\
+         prod_comp p x (prod_op p y z) /\
+         prod_op p x (prod_op p y z) == prod_op p (prod_op p x y) z)
+let prod_assoc_r #a p x y z =
+  let aux w : 
     Lemma (composable (p w) (y w) (z w) /\
-           composable (p w) (x w) (op (p w) (y w) (z w)) /\
-           op (p w) (x w) (op (p w) (y w) (z w)) == op (p w) (op (p w) (x w) (y w)) (z w)) 
-  = (p w).assoc_r (x w) (y w) (z w) in
-  forall_intro assoc_r;
-  ext a f (prod_op f p x (prod_op f p y z)) (prod_op f p (prod_op f p x y) z)
+           composable (p w) (x w) (op (p w) (y w) (z w)))
+    [SMTPat (p w)] = (p w).assoc_r (x w) (y w) (z w)
+  in
+  ext (prod_op p x (prod_op p y z)) (prod_op p (prod_op p x y) z)
+    (fun w -> (p w).assoc (x w) (y w) (z w))
 
 val prod_is_unit :
-  f:('a -> Type) -> p:(z:'a -> pcm (f z)) ->
+  #f:('a -> Type) -> p:(z:'a -> pcm (f z)) ->
   x:restricted_t 'a f ->
-  Lemma (prod_comp f p x (prod_one f p) /\
-         prod_op f p x (prod_one f p) == x)
-let prod_is_unit #a f p x =
-  let is_unit (y:a): 
-    Lemma (composable (p y) (x y) (prod_one f p y) /\
-           op (p y) (x y) (prod_one f p y) == x y)
-  = (p y).is_unit (x y) in
-  forall_intro is_unit;
-  ext a f (prod_op f p x (prod_one f p)) x
+  Lemma (prod_comp p x (prod_one p) /\
+         prod_op p x (prod_one p) == x)
+let prod_is_unit #a p x =
+  let is_unit y :
+    Lemma (composable (p y) (x y) (prod_one p y))
+    [SMTPat (p y)] = (p y).is_unit (x y)
+  in ext (prod_op p x (prod_one p)) x (fun y -> (p y).is_unit (x y))
 
-val prod_pcm : f:('a -> Type) -> (z:'a -> pcm (f z)) -> pcm (restricted_t 'a f)
-let prod_pcm #a f p = FStar.PCM.({
-  p = prod_pcm' f p;
-  comm = prod_comm f p;
-  assoc = prod_assoc f p;
-  assoc_r = prod_assoc_r f p;
-  is_unit = prod_is_unit f p;
-  refine = (fun x ->
-    (forall z. x z == (p z).p.one) \/
-    (forall z. (p z).refine (x z) /\ ~ (x z == (p z).p.one)))
-})
+val prod_refine :
+  #f:('a -> Type) -> (y:'a -> pcm (f y)) ->
+  x: restricted_t 'a f -> prop
+let prod_refine p x = forall y. (p y).refine (x y)
+
+val prod_pcm : #f:('a -> Type) -> (z:'a -> pcm (f z)) -> pcm (restricted_t 'a f)
+let prod_pcm #a #f p = {
+  p = {composable = prod_comp p; op = prod_op p; one = prod_one p};
+  comm = prod_comm p;
+  assoc = prod_assoc p;
+  assoc_r = prod_assoc_r p;
+  is_unit = prod_is_unit p;
+  refine = prod_refine p
+}
 
 /// Similarly, given a PCM for each z:a, we can model a-ary unions with an PCM for option (x:a & f x), where
 /// - None is the unit of the PCM
@@ -386,11 +262,7 @@ let union_op f p x y = match x, y with
 
 val union_pcm : f:('a -> Type) -> p:(x: 'a -> pcm (f x)) -> pcm (union 'a f p)
 let union_pcm #a f p = FStar.PCM.({
-  p = {
-    composable=union_comp f p;
-    op=union_op f p;
-    one=None
-  };
+  p = {composable = union_comp f p; op = union_op f p; one = None};
   comm = (fun x y -> match x, y with
     | None, _ | _, None -> ()
     | Some (|xa, xb|), Some (|ya, yb|) -> (p xa).comm xb yb);
@@ -401,113 +273,11 @@ let union_pcm #a f p = FStar.PCM.({
     | None, _, _ | _, _, None | _, None, _ -> ()
     | Some (|xa, xb|), Some (|ya, yb|), Some (|za, zb|) -> (p xa).assoc_r xb yb zb);
   is_unit = (fun _ -> ());
-  refine = (fun x -> match x with
-    | None -> True
-    | Some (|xa, xb|) -> (p xa).refine xb /\ ~(xb == (p xa).p.one))
+  refine = (fun x -> match x with None -> True | Some (|xa, xb|) -> (p xa).refine xb)
 })
 
-
 (*
-val upd_gen (#a:Type) (#p:pcm a) (r:ref a p) (x y:Ghost.erased a)
-            (f:FStar.PCM.frame_preserving_upd p x y)
-  : SteelT unit
-           (pts_to r x)
-           (fun _ -> pts_to r y)
-           *)
-
-(*
-let upd_first #a #b (r:ref (t a b) pcm_t) (x:Ghost.erased a) (y:a)
-  : SteelT unit (pts_to r (First #a #b x)) (fun _ -> pts_to r (First #a #b y))
-= let f : frame_preserving_upd_0 pcm_t (Ghost.hide (First #a #b x)) (First #a #b y) =
-    fun old_v ->
-      match old_v with
-      | First _ -> First y
-      | Both _ z -> Both y z
-  in
-  change_slprop (pts_to r (First (Ghost.reveal x))) (pts_to r (Ghost.reveal (Ghost.hide (First (Ghost.reveal x))))) (fun _ -> ());
-  upd_gen r (Ghost.hide (First #a #b x)) (Ghost.hide (First #a #b y)) f;
-  change_slprop (pts_to r (Ghost.reveal (Ghost.hide (First y)))) (pts_to r (First y)) (fun _ -> ())
-  *)
-
-(*
-val prod_upd :
-  #a:eqtype -> f:(a -> Type) -> 
-  field:a -> y: f field -> xs: restricted_t a f -> 
-  restricted_t a f
-let prod_upd #a f field y xs =
-  on_domain a (fun field' -> if field = field' then y else xs field')
-
-let frame_preserving_upd #a (p:pcm a) (x y:a) =
-  f: (v:a{compatible p x v}
-      -> Tot (z:a{
-                compatible p y z /\
-                 (p.refine v ==> p.refine z) /\
-                 (p.refine v ==> frame_preserving p v z)}))
-  {
-     forall (v:a{compatible p x v}).
-         let z = f v in
-         (forall (frame:a). {:pattern (composable p v frame)}
-              composable p v frame ==>
-              composable p z frame /\
-              (compatible p x (op p v frame) ==> (op p z frame == f (op p v frame))))
-  }
-
-val frame_preserving_upd_field :
-  #a:eqtype -> f:(a -> Type) -> p:(field:a -> pcm (f field)) ->
-  field:a -> x: f field -> y: f field ->
-  xs: restricted_t a f {xs field == x} ->
-  frame_preserving_upd (p field) x y ->
-  frame_preserving_upd (prod_pcm f p) xs (update f field y xs)
-let frame_preserving_upd_field #a f p field x y xs upd =
-  _
-  *)
-
-(*
-val update : ...
-
-val upd_field :
-  f:('a -> Type) -> p:(z:'a -> pcm (f z)) ->
-  r:ref (restricted_t 'a f) (prod_pcm f p) ->
-  field: 'a -> values: Ghost.erased (restricted_t 'a f{defined only at one field}) ->
-  x: Ghost.erased (f field) -> y: f field ->
-  (frame_preserving_upd_0 (p field) x y) ->
-  SteelT unit (pts_to r (Ghost.reveal values))
-              (fun _ -> pts_to r (update field y values))
-
-let upd_first #a #b (r:ref (t a b) pcm_t) (x:Ghost.erased a) (y:a)
-  : SteelT unit (pts_to r (First #a #b x)) (fun _ -> pts_to r (First #a #b y))
-let f : frame_preserving_upd_0 pcm_t (Ghost.hide (First #a #b x)) (First #a #b y) = fun old_v ->
-    match old_v with
-    | First _ -> First y
-    | Both _ z -> Both y z
-in change_slprop (pts_to r (First (Ghost.reveal x))) (pts_to r (Ghost.reveal (Ghost.hide (First (Ghost.reveal x))))) (fun _ -> ());
-   upd_gen r (Ghost.hide (First #a #b x)) (Ghost.hide (First #a #b y)) f;
-   change_slprop (pts_to r (Ghost.reveal (Ghost.hide (First y)))) (pts_to r (First y)) (fun _ -> ())
-
-
-let upd_first #a #b (r:ref (t a b) pcm_t) (x:Ghost.erased a) (y:a)
-  : SteelT unit (pts_to r (First #a #b x)) (fun _ -> pts_to r (First #a #b y))
-= let f : frame_preserving_upd_0 pcm_t (Ghost.hide (First #a #b x)) (First #a #b y) = fun old_v ->
-    match old_v with
-    | First _ -> First y
-    | Both _ z -> Both y z
-in change_slprop (pts_to r (First (Ghost.reveal x))) (pts_to r (Ghost.reveal (Ghost.hide (First (Ghost.reveal x))))) (fun _ -> ());
-   upd_gen r (Ghost.hide (First #a #b x)) (Ghost.hide (First #a #b y)) f;
-   change_slprop (pts_to r (Ghost.reveal (Ghost.hide (First y)))) (pts_to r (First y)) (fun _ -> ())
-
-
-let upd_first #a #b (r:ref (t a b) pcm_t) (x:Ghost.erased a) (y:a)
-  : SteelT unit (pts_to r (First #a #b x)) (fun _ -> pts_to r (First #a #b y))
-= let f : frame_preserving_upd_0 pcm_t (Ghost.hide (First #a #b x)) (First #a #b y) = fun old_v ->
-    match old_v with
-    | First _ -> First y
-    | Both _ z -> Both y z
-in change_slprop (pts_to r (First (Ghost.reveal x))) (pts_to r (Ghost.reveal (Ghost.hide (First (Ghost.reveal x))))) (fun _ -> ());
-   upd_gen r (Ghost.hide (First #a #b x)) (Ghost.hide (First #a #b y)) f;
-   change_slprop (pts_to r (Ghost.reveal (Ghost.hide (First y)))) (pts_to r (First y)) (fun _ -> ())
-
-
-// TODO frame-preserving updates
+// TODO
 // move 2d point along x
 // move 2d point along y
 // given a function "incrementX" and "incrementY"; write a function that calls it in a loop
